<?xml version="1.0" encoding="UTF-8"?>
<!DOCTYPE rdf:RDF [
        <!ENTITY rdf  "http://www.w3.org/1999/02/22-rdf-syntax-ns#">
        <!ENTITY rdfs "http://www.w3.org/2000/01/rdf-schema#">
        <!ENTITY skos "http://www.w3.org/2004/02/skos/core#">
        <!ENTITY dc   "http://purl.org/dc/terms/">
        <!ENTITY owl  "http://www.w3.org/2002/07/owl#">
        <!ENTITY xs   "http://www.w3.org/2001/XMLSchema#">
        <!ENTITY wwct "http://brightbyte.de/vocab/wikiword/concept-type#">
        <!ENTITY ww   "http://brightbyte.de/vocab/wikiword#">
        <!ENTITY this "http://brightbyte.de/vocab/wikiword">
]>

<rdf:RDF
	xmlns:rdf=  "&rdf;" 
	xmlns:rdfs= "&rdfs;"
	xmlns:skos= "&skos;"
	xmlns:dc=   "&dc;"
	xmlns:owl=  "&owl;"
	xmlns:ww=   "&ww;"
	xmlns:xs=   "&xs;"
	xml:base=   "&this;"> 

<rdf:Description rdf:about="">
    <dc:title xml:lang="en">WikiWord schema for RDF, based on SKOS</dc:title>
    <dc:contributor>Daniel Kinzler</dc:contributor>
    <dc:publisher>Universit&#x00E4;t Leipzig</dc:publisher>
    <dc:references rdf:resource="http://www.w3.org/2004/02/skos/core"/>
    <rdfs:comment>Created as part of the diploma thesis 
    &quot;Automatischer Aufbau eines multilingualen Thesaurus durch
    Extraktion semantischer und lexikalischer Relationen aus Wikipedia&quot;
    to be completed in April 2008
    </rdfs:comment>
</rdf:Description>

<rdf:Property rdf:ID="similar">
    <rdfs:label xml:lang="en">similar to</rdfs:label>
    <rdfs:label xml:lang="de">&#x00E4;hnlich zu</rdfs:label>
    <rdfs:subPropertyOf rdf:resource="&skos;related"/>
    <skos:definition xml:lang="en">A concept which is semantically similar.
    </skos:definition>
    <skos:definition xml:lang="de">Ein semantisch &#x00E4;hnliches Konzept.
    </skos:definition>
    <rdfs:isDefinedBy rdf:resource="&this;"/>
    <rdfs:comment xml:lang="en">This is stronger than skos:related, and
    intended for concepts that are &quot;nearly the same&quot;.
    </rdfs:comment>
</rdf:Property>

<rdf:Property rdf:ID="assoc">
    <rdfs:label xml:lang="en">associated with</rdfs:label>
    <rdfs:label xml:lang="de">assoziiert mit</rdfs:label>
    <rdfs:subPropertyOf rdf:resource="&skos;semanticRelation"/>
    <skos:definition xml:lang="en">A concept which is somehow associated.
    </skos:definition>
    <skos:definition xml:lang="de">Ein irgendwie assoziiertes Konzept.
    </skos:definition>
    <rdfs:isDefinedBy rdf:resource="&this;"/>
    <rdfs:comment xml:lang="en">This is weaker than skos:related, and not
    required to by symmetric.
    </rdfs:comment>
</rdf:Property>

<rdf:Property rdf:ID="type">
    <rdfs:label xml:lang="en">concept type</rdfs:label>
    <rdfs:label xml:lang="de">Konzepttyp</rdfs:label>
    <rdf:type rdf:resource="&rdf;Property"/> 
    <rdfs:range rdf:resource="&ww;concept-type"/>
    <rdfs:domain rdf:resource="&skos;Concept"/>
    <skos:definition xml:lang="en">The concept&amp;s type.</skos:definition>
    <skos:definition xml:lang="de">Typ des Konzepts.</skos:definition>
    <rdfs:isDefinedBy rdf:resource="&this;"/>
    <rdfs:comment xml:lang="en">May be useful to filter proper nouns from
    common nounds, fetch only locations, etc. Standard values are defined
    in the namespace &this;/concept-type#, namely UNKNOWN, PLACE,
    PERSON,	ORGANISATION, NAME,	TIME, NUMBER, LIFEFORM,	OTHER; other values
    are allowed. 
    </rdfs:comment>
</rdf:Property>
	
<rdf:Property rdf:ID="displayLabel">
    <rdfs:label xml:lang="en">display label</rdfs:label>
    <rdfs:subPropertyOf rdf:resource="&rdfs;label"/>
    <rdfs:domain rdf:resource="&skos;Concept"/>
    <skos:definition xml:lang="en">The suggested display label for a resource,
    in a given language.
    </skos:definition>
    <skos:definition xml:lang="de">Der vorgeschlagene Anzeigename einer
    Ressource, in einer bestimmten Sprache.
    </skos:definition>
    <rdfs:comment xml:lang="en">No two concepts in the same concept scheme may
    have the same value for ww:displayLabel in a given language. However, in
    contrast to prefLabel, the value of the displayLable may be re-occurr as a
    prefLabel, altLable or hiddenLabel. Also in contrast to prefLabel, a
    displayLable may not be a naturally occurring term used to reference the
    concept in question in natural language: specifically, it may be
    artificially disambiguated.
    </rdfs:comment>
    <rdfs:isDefinedBy rdf:resource="&this;"/>
</rdf:Property>
	
<rdf:Property rdf:ID="score">
    <rdfs:label xml:lang="en">score</rdfs:label>
    <rdfs:subPropertyOf rdf:resource="&rdfs;label"/>
    <rdfs:range rdf:resource="&xs;decimal"/> 
    <rdfs:comment xml:lang="en">Basis for any scores to be associated with a concept, term or relation.
    </rdfs:comment>
    <rdfs:isDefinedBy rdf:resource="&this;"/>
</rdf:Property>
	
<rdf:Property rdf:ID="rank">
    <rdfs:label xml:lang="en">rank</rdfs:label>
    <rdfs:subPropertyOf rdf:resource="&rdfs;label"/>
    <rdfs:range rdf:resource="&xs;integer"/> 
    <rdfs:comment xml:lang="en">Basis for any ranks to be associated with a concept, term or relation.
    Note that ranks are positive integers, and required to be unique within one scheme/corpus.
    </rdfs:comment>
    <rdfs:isDefinedBy rdf:resource="&this;"/>
</rdf:Property>
	
<rdf:Property rdf:ID="idfScore">
    <rdfs:label xml:lang="en">Inverse Document Frequency</rdfs:label>
    <rdfs:subPropertyOf rdf:resource="&ww;score"/>
    <rdfs:domain rdf:resource="&skos;Concept"/>
    <skos:definition xml:lang="en">The Inverse Document Frequency Score of a concept, 
    as derived from the incomming hyperlinks to the documents that define it.
    </skos:definition>
    <rdfs:comment xml:lang="en">The IDF is an indicator for the selectiveness of a concept.
    See "Introduction to Modern Information
    Retrieval" (Salton 1986) for a definietion of Inverse Document Frequency.
    </rdfs:comment>
    <rdfs:isDefinedBy rdf:resource="&this;"/>
</rdf:Property>
	
<rdf:Property rdf:ID="lhsScore">
    <rdfs:label xml:lang="en">Local Hierarchy Score</rdfs:label>
    <rdfs:subPropertyOf rdf:resource="&ww;score"/>
    <rdfs:domain rdf:resource="&skos;Concept"/>
    <skos:definition xml:lang="en">The Local Hierarchy Score of a concept, 
    as derived from the incomming and outgoing hyperlinks of the documents that define it.
    </skos:definition>
    <rdfs:comment xml:lang="en">The LHS is an indicator for the centrality of a concept.
    See "Self-emergence of knowledge trees: Extraction of the
    Wikipedia hierarchies" (Muchnik et.Al. 2007) for a definietion of  Local Hierarchy
    Score. The version of the formula used by WikiWord does not include a symmetrical
    counterpart.
    </rdfs:comment>
    <rdfs:isDefinedBy rdf:resource="&this;"/>
</rdf:Property>

<rdf:Property rdf:ID="inDegree">
    <rdfs:label xml:lang="en">In-Degree</rdfs:label>
    <rdfs:subPropertyOf rdf:resource="&ww;score"/>
    <rdfs:domain rdf:resource="&skos;Concept"/>
    <skos:definition xml:lang="en">Node degree with respect to incomming links.</skos:definition>
    <rdfs:isDefinedBy rdf:resource="&this;"/>
</rdf:Property>

<rdf:Property rdf:ID="outDegree">
    <rdfs:label xml:lang="en">Out-Degree</rdfs:label>
    <rdfs:subPropertyOf rdf:resource="&ww;score"/>
    <rdfs:domain rdf:resource="&skos;Concept"/>
    <skos:definition xml:lang="en">Node degree with respect to outgoing links.</skos:definition>
    <rdfs:isDefinedBy rdf:resource="&this;"/>
</rdf:Property>

<rdf:Property rdf:ID="linkDegree">
    <rdfs:label xml:lang="en">Link-Degree</rdfs:label>
    <rdfs:subPropertyOf rdf:resource="&ww;score"/>
    <rdfs:domain rdf:resource="&skos;Concept"/>
    <skos:definition xml:lang="en">Node degree with respect to incomming and outgoing links combined.</skos:definition>
    <rdfs:isDefinedBy rdf:resource="&this;"/>
</rdf:Property>


<rdf:Property rdf:ID="idfRank">
    <rdfs:label xml:lang="en">IDF Rank</rdfs:label>
    <rdfs:subPropertyOf rdf:resource="&ww;rank"/>
    <rdfs:domain rdf:resource="&skos;Concept"/>
    <skos:definition xml:lang="en">Rank with respect to the idfScore.</skos:definition>
    <rdfs:isDefinedBy rdf:resource="&this;"/>
</rdf:Property>

<rdf:Property rdf:ID="lhsRank">
    <rdfs:label xml:lang="en">LHS Rank</rdfs:label>
    <rdfs:subPropertyOf rdf:resource="&ww;rank"/>
    <rdfs:domain rdf:resource="&skos;Concept"/>
    <skos:definition xml:lang="en">Rank with respect to the lhsScrore.</skos:definition>
    <rdfs:isDefinedBy rdf:resource="&this;"/>
</rdf:Property>
	
<rdf:Property rdf:ID="inRank">
    <rdfs:label xml:lang="en">In-Degree Rank</rdfs:label>
    <rdfs:subPropertyOf rdf:resource="&ww;rank"/>
    <rdfs:domain rdf:resource="&skos;Concept"/>
    <skos:definition xml:lang="en">Rank with respect to the inDegree.</skos:definition>
    <rdfs:isDefinedBy rdf:resource="&this;"/>
</rdf:Property>
	
<rdf:Property rdf:ID="outRank">
    <rdfs:label xml:lang="en">Out-Degree Rank</rdfs:label>
    <rdfs:subPropertyOf rdf:resource="&ww;rank"/>
    <rdfs:domain rdf:resource="&skos;Concept"/>
    <skos:definition xml:lang="en">Rank with respect to the outDegree.</skos:definition>
    <rdfs:isDefinedBy rdf:resource="&this;"/>
</rdf:Property>
	
<rdf:Property rdf:ID="linkRank">
    <rdfs:label xml:lang="en">Link-Degree Rank</rdfs:label>
    <rdfs:subPropertyOf rdf:resource="&ww;rank"/>
    <rdfs:domain rdf:resource="&skos;Concept"/>
    <skos:definition xml:lang="en">Rank with respect to the linkDegree.</skos:definition>
    <rdfs:isDefinedBy rdf:resource="&this;"/>
</rdf:Property>

<rdfs:Class rdf:ID="concept-type">
  <rdfs:label xml:lang="en">concept type</rdfs:label>
  <skos:definition xml:lang="en">The type of a concept</skos:definition>
</rdfs:Class>

<rdf:Description rdf:about="&wwct;UNKNOWN">
	<rdf:type>&ww;concept-type</rdf:type>
    <rdfs:label xml:lang="en">unknown</rdfs:label>
    <skos:definition xml:lang="en">Unknown concept type, indicating that no information is avialable about the concept.
	 If some information is avialable, but not specific type could be assigned, the type OTHER</skos:definition>
    <rdfs:isDefinedBy rdf:resource="&this;"/>
</rdf:Description>
	
<rdf:Description rdf:about="&wwct;PLACE">
	<rdf:type>&ww;concept-type</rdf:type>
    <rdfs:label xml:lang="en">place</rdfs:label>
    <skos:definition xml:lang="en">A geographic location; This type SHOULD NOT be used for specific buildings or simmilar
	 sites that merely have a geographic location. </skos:definition>
    <rdfs:isDefinedBy rdf:resource="&this;"/>
</rdf:Description>
	
<rdf:Description rdf:about="&wwct;PERSON">
	<rdf:type>&ww;concept-type</rdf:type>
    <rdfs:label xml:lang="en">person</rdfs:label>
    <skos:definition xml:lang="en"> A person (MAY be fictional, SHOULD be human if not fictional). </skos:definition>
    <rdfs:isDefinedBy rdf:resource="&this;"/>
</rdf:Description>
	
<rdf:Description rdf:about="&wwct;ORGANISATION">
	<rdf:type>&ww;concept-type</rdf:type>
    <rdfs:label xml:lang="en">organisation</rdfs:label>
    <skos:definition xml:lang="en">An organisation, loke a cooperation or NGO, a union, etc. This 
	 MAY include government organisations, but not states as such. </skos:definition>
    <rdfs:isDefinedBy rdf:resource="&this;"/>
</rdf:Description>
	
<rdf:Description rdf:about="&wwct;NAME">
	<rdf:type>&ww;concept-type</rdf:type>
    <rdfs:label xml:lang="en">name</rdfs:label>
    <skos:definition xml:lang="en">A name as such, i.e. a first name or last name.</skos:definition>
    <rdfs:isDefinedBy rdf:resource="&this;"/>
</rdf:Description>
	
<rdf:Description rdf:about="&wwct;TIME">
	<rdf:type>&ww;concept-type</rdf:type>
    <rdfs:label xml:lang="en">time</rdfs:label>
    <skos:definition xml:lang="en">A point in time, or time period, like "17th century". Recurrent dates (like "March 3rd") 
	 MAY also have this type. Concepts that go beyond a pure notion of time or date (like "Monday"
	 or "9/11") SHOULD NOT have this type.</skos:definition>
    <rdfs:isDefinedBy rdf:resource="&this;"/>
</rdf:Description>
	
<rdf:Description rdf:about="&wwct;NUMBER">
	<rdf:type>&ww;concept-type</rdf:type>
    <rdfs:label xml:lang="en">number</rdfs:label>
    <skos:definition xml:lang="en">A number, like "three". Special constants like Pi or e MAY also have this type.
	 Concepts that go beyond a pure notion of a number (like "dozen") 
	 SHOULD NOT have this type. </skos:definition>
    <rdfs:isDefinedBy rdf:resource="&this;"/>
</rdf:Description>
	
<rdf:Description rdf:about="&wwct;LIFEFORM">
	<rdf:type>&ww;concept-type</rdf:type>
    <rdfs:label xml:lang="en">life form</rdfs:label>
    <skos:definition xml:lang="en">Biological taxon describing a life form (i.e. a genus, a species, etc).</skos:definition>
    <rdfs:isDefinedBy rdf:resource="&this;"/>
</rdf:Description>
	
<rdf:Description rdf:about="&wwct;OTHER">
	<rdf:type>&ww;concept-type</rdf:type>
    <rdfs:label xml:lang="en">other</rdfs:label>
    <skos:definition xml:lang="en">Unknown concept type. Generic catch all type, expected to occurr frequently.</skos:definition>
    <rdfs:isDefinedBy rdf:resource="&this;"/>
</rdf:Description>
	
<!--<rdf:Description rdf:about="&wwct;ALIAS">
	<rdf:type>&ww;concept-type</rdf:type>
    <rdfs:label xml:lang="en">unknown</rdfs:label>
    <skos:definition xml:lang="en"></skos:definition>
    <rdfs:isDefinedBy rdf:resource="&this;"/>
</rdf:Description>-->
	
</rdf:RDF>